moving modDiv from method to function

dafny/cycle.dfy
@@ -1,99 +1,132 @@
-include "mod.dfy"
+include "modDiv.dfy"
 
 /**
  * Define the cycle function
  * Ensure some important properties into the cycle function
- * assert forall k: nat :: |source| <= k  < |dest|  ==> Mod.mod(k,|source|) < |source|;
- * assert forall k: nat :: |source| <= k  < |dest|  ==> dest[k] == source[Mod.mod(k,|source|)];
+ * assert forall k: nat :: |source| <= k  < |dest|  ==> ModDiv.mod(k,|source|) < |source|;
+ * assert forall k: nat :: |source| <= k  < |dest|  ==> dest[k] == source[ModDiv.mod(k,|source|)];
  * assert forall k: nat :: |source| <= k  < |dest|  ==> dest[k] == dest[k-|source|];
  */
 module Cycle {
 
-    import Mod
+    import ModDiv
 
-    function method cyclePos(list: seq<nat>, pos: nat): nat
+    function method isCycle(list: seq<nat>, listCycle: seq<nat>): bool
         requires |list| > 0;
+//        requires |listCycle| >= |list|;
     {
-        var l := |list|;
-        var k := Mod.mod(pos, l);
-        Mod.remainderShouldBeSmall(pos,l,k);
-        assert k < l;
-        var result := list[k];
-        result
+        var limit := if |listCycle| > |list| then |list| else |listCycle|;
+        var equalsFirst    := listCycle[..limit] == list;
+        var equalsPrevious := forall k : nat :: |list| <= k < |listCycle| ==> listCycle[k] == listCycle[k - |list|];
+        var equalsMod      := forall k : nat :: 0      <= k < |listCycle| ==> listCycle[k] == list[ k % |list| ];
+
+        assert equalsFirst    ==> listCycle[..limit] == list[..limit];
+        assert equalsPrevious ==> forall k : nat :: |list| <= k < |listCycle| ==> listCycle[k] == listCycle[k - |list|];
+        assert equalsMod      ==> forall k : nat :: 0      <= k < |listCycle| ==> listCycle[k] == list[ k % |list| ];
+
+        equalsFirst && equalsPrevious && equalsMod
     }
 
-    lemma checkCyclePos(list: seq<nat>, pos: nat, key: nat, result: nat)
+    method cycleUntil(list:seq<nat>, size: nat, gap: nat) returns (result: seq<nat>) 
         requires |list| > 0;
-        requires key == Mod.mod(pos,|list|);
-        requires result == cyclePos(list, pos);
-        ensures key < |list|;
-        ensures result == list[key];
-    {
-        Mod.remainderShouldBeSmall(pos,|list|,key);
-    }
-
-    method cycle(source: seq<nat>, size: nat) returns (result: seq<nat>)
-        requires |source| > 0;
-        ensures forall k : nat :: 0 <= k < |result| ==> Mod.mod(k,|source|) < |source|;
-        ensures forall k : nat :: 0 <= k < |result| ==> result[k] == source[Mod.mod(k,|source|)];
+        requires size >= |list|;
         ensures |result| == size;
+        ensures isCycle(list, result);
+        decreases size;
     {
-        result := [];   
-        while( |result| < size ) 
-            invariant forall k : nat :: 0 <= k < |result| ==> result[k] == source[Mod.mod(k,|source|)];
-            invariant |result| <= size;
-            decreases size - |result|;
+        var arr := new nat[size];
+        var key := 0;
+        var modKey := 0;
+        while ( key < size )
+            decreases size - key;
+            invariant key <= size;
+            invariant key > 0 ==> isCycle(list, arr[..key]);
         {
-            var value := cyclePos(source, |result|);            
-            result := result + [value];
+            var mod, div := ModDiv.modDiv(key,|list|);
+            assert ModDiv.isModDiv(key,|list|,mod,div);
+            if ( key < |list| ) {
+                ModDiv.modSmallValues(key,|list|,mod,div);
+                assert modKey < |list| ==> modKey == key;
+            }
+            arr[key] := list[modKey];
+            assert key < |list| ==> arr[..key] == list[..key];
+            if ( key >= |list| ) {
+                ModDiv.isModDivMinus(key,|list|,mod,div);
+            }
+            assert forall k : nat :: |list| <= k < key ==> arr[k] == arr[k - |list|];
+            assert forall k : nat :: 0      <= k < key ==> arr[k] == list[ k % |list| ];
+            key := key + 1;
         }
-        assert |result| == size;
+        assert key == size;
+        result := arr[..];
+
+        // if (size == 0 ) {
+        //     result := [];
+        //     return;
+        // } else {
+        //     var key := ModDiv.mod(gap,|list|);
+        //     assert key < |list|;
+        //     var current := list[key];
+        //     var others := cycleUntil(list, size - 1, gap + 1);
+        //     result := [current] + others;
+        // }
+    }
+    
+    lemma modIscycle(list: seq<nat>, listCycle: seq<nat>)
+        requires |list| > 0;
+        requires forall k : nat :: 0 <= k < |listCycle| ==> listCycle[k] == list[k % |list|];
+        ensures isCycle(list, listCycle);
+    {
+        var limit := if |listCycle| > |list| then |list| else |listCycle|;
+        assert forall k : nat :: 0      <= k < |listCycle| ==> ModDiv.isMod(k, |list|, k % |list|);
+        // assert listCycle[..limit] == list[..limit];
+        assert forall k : nat :: |list| <= k < |listCycle| ==> listCycle[k] == listCycle[k - |list|];
+        assert forall k : nat :: 0      <= k < |listCycle| ==> listCycle[k] == list[ k % |list| ];
+
     }
 
-    function isCycle(list: seq<nat>, listCycle: seq<nat>): bool
+    /**
+     * Since the current definition of the cycle mod is alligned with the definition of the isModDiv
+     * all the properties defined to the isModDiv can be applied to the cycle.
+     */
+    lemma cycleIsMod(list: seq<nat>, listCycle: seq<nat>)
         requires |list| > 0;
         requires |listCycle| >= |list|;
+        requires isCycle(list, listCycle);
+        ensures forall k : nat :: 0 <= k < |listCycle| ==> ModDiv.isModDiv(k, |list|, k / |list|, k % |list|);
     {
-        assert forall k : nat :: |list| <= k < |listCycle| ==> Mod.mod(k,|list|) == Mod.mod(k - |list|,|list|);
-        assert forall k : nat :: 0 <= k < |list| ==> Mod.mod(k,|list|) == k;
-        forall k : nat :: 0 <= k < |listCycle| ==> listCycle[k] == list[Mod.mod(k,|list|)]
+        assert forall k : nat :: 0 <= k < |listCycle| ==> listCycle[k] == list[ k % |list| ];
+        assert forall k : nat :: 0 <= k < |listCycle| ==> ModDiv.isModDiv(k, |list|, k / |list|, k % |list|);
     }
 
-    method checkCycle(source: seq<nat>, m: nat)
-        requires |source| > 0;
+    lemma cycleShouldContainsList(list: seq<nat>, cycleList: seq<nat>)
+        requires |list| > 0;
+        requires |cycleList| >= |list|;
+        requires isCycle(list, cycleList);
+        ensures cycleList[0..|list|] == list;
+    {
+    }
+
+    lemma cycleByConcat(list: seq<nat>, cycleList: seq<nat>, smallCycle: seq<nat>, m: nat)
+        requires |list| > 0;
+        requires |cycleList| > |list|;
+        requires |smallCycle| > |list|;
+        requires isCycle(list, cycleList);
+        requires isCycle(list, smallCycle);
+        requires |cycleList| == |list| * m;
+        requires |smallCycle| == |cycleList| - |list|;
+        requires |smallCycle| == |list| * ( m - 1 );
         requires m > 0;
+        ensures cycleList == list + cycleList[|list|..];
+        ensures cycleList == list + smallCycle;
     {
-        var dest := cycle( source, |source| * m);
-        assert |dest| == |source| * m;
-        assert forall k: nat :: 0 <= k < |source|  ==> dest[k] == source[k];
-        assert forall k: nat :: |source| <= k  < |dest|  ==> Mod.mod(k,|source|) < |source|;
-        assert forall k: nat :: |source| <= k  < |dest|  ==> dest[k] == source[Mod.mod(k,|source|)];
-        assert forall k: nat :: |source| <= k  < |dest|  ==> dest[k] == dest[k-|source|];
+        assert cycleList[0..|list|] == list;
     }
 
-    method test()
-    {
-        var source := [1,2,3];
-        checkCycle(source,2);
-        var dest := cycle(source,7);
-        assert |dest| == 7;
-        assert forall k: nat :: |source| <= k  < |dest|  ==> Mod.mod(k,|source|) < |source|;
-        assert forall k: nat :: |source| <= k  < |dest|  ==> dest[k] == source[Mod.mod(k,|source|)];
-        assert forall k: nat :: |source| <= k  < |dest|  ==> dest[k] == dest[k-|source|];
-        assert |source| == 3;
-        assert dest[0] == dest[3] == dest[6] == source[0];
-        assert dest[1] == dest[4] == source[1];
-        assert dest[2] == dest[5] == source[2];
-        assert source == [1,2,3];
-        assert dest == [1,2,3,1,2,3,1];
-        print("dest = ");
-        print(dest);
-    }
-
-    // method Main()
-    // {
-    //     print("\ntesting cycle\n");
-    //     test();
-    //     print("\n:D\n");
-    // }
+//     method Main()
+//     {
+//         print("\ntesting cycle\n");
+//         print(isCycle([1,2,3],[1,2,3,1,2,3,1,4]));
+//         print("\n:D\n");
+//     }
 }
