dafny/old/Readme.md
@@ -1,0 +1,3 @@
+# Old versions
+
+Some different ways to define the same mathematic functions that we are not using anymore considering some issues around using them to create some proofs.
